AvgCaseMls.lean
@@ -1,4 +1,5 @@
 import AvgCaseMls.MLS
+import AvgCaseMls.EMLS
 import AvgCaseMls.DecideMLS
 import AvgCaseMls.AvCom
 import AvgCaseMls.AverageHardness
